Going to try a thing

theories/embeddingOneTypeLevel.v
@@ -2,31 +2,23 @@ Require Import String.
 Require Import qterm.
 Require Import lambdaFacts.
 Require Import lambdaSolve.
-
-(*
-Here I will use the library to define dependent type theory.
-For now, I'll just do type : type.
-*)
-
-
-(* The shallow embedding. Ideally this would work with nice notations, but for now Definitions: *)
+Require Import FunctionalExtensionality.
+Require Import Coq.Logic.PropExtensionality.
 
 Definition nil := <Nil>.
-Definition cons := <fun gamma => fun ty => cons gamma ty>.
+Definition cons := <fun env => fun ty => cons env ty>.
 
-Definition zero := <fun x => proj2 x>.
-Definition succ := <fun x => fun gamma => x (proj1 gamma)>.
+Definition zero := <fun env => proj2 env>.
+Definition succ := <fun x => fun env => x (proj1 env)>.
 
-Definition lzero := <lzero>.
-Definition lsuc := <lsuc>.
-Definition pi := <fun x => fun y => fun gamma => Pi (x gamma) (fun a => y (gamma , a))>.
+Definition pi := <fun x => fun y => fun env => Pi (x env) (fun a => y (env , a))>.
 Definition U : QTerm := <fun env => U>.
 Definition Empty := <fun env => Empty>.
 Definition Bool := <fun env => Bool>.
 
 Definition var_to_term := <fun x => x>.
-Definition lambda := <fun t => fun gamma => fun a => t (gamma , a)>.
-Definition app := <fun t1 => fun t2 => fun gamma => (t1 gamma) (t2 gamma)>.
+Definition lambda := <fun t => fun env => fun a => t (env , a)>.
+Definition app := <fun t1 => fun t2 => fun env => (t1 env) (t2 env)>.
 Definition true := <fun env => fun p => proj1 p>.
 Definition false := <fun env => fun p => proj2 p>.
 Definition ifexpr := <fun cond => fun t1 => fun t2 => fun env => (cond env) (t1 env, t2 env)>.
@@ -35,15 +27,14 @@ Definition weaken := <fun t => fun env => t (proj1 env)>.
 Definition subLast := <fun t => fun toSub => fun env => t (env , toSub env)>.
 
 Ltac unfold_all := unfold nil, cons, zero, succ, pi, U, Bool, Empty, var_to_term, lambda,
-    app, weaken, subLast, lzero, lsuc, true, false, ifexpr in *.
+    app, weaken, subLast, true, false, ifexpr in *.
 
 (* The deeper shallow embedding *)
 
 Inductive VarTyped : QTerm -> QTerm -> QTerm -> Prop :=
 | ty_zero : forall ctx T, VarTyped <`cons `ctx `T> <`weaken `T> zero
 | ty_succ : forall ctx A T s, VarTyped ctx A s
-                              -> VarTyped <`cons `ctx `T> <`weaken `A> <`succ `s>
-.
+                              -> VarTyped <`cons `ctx `T> <`weaken `A> <`succ `s>.
 
 Inductive Typed : QTerm -> QTerm -> QTerm -> Prop :=
 | ty_lambda : forall ctx A B s,
@@ -59,14 +50,11 @@ Inductive Typed : QTerm -> QTerm -> QTerm -> Prop :=
     Typed ctx <`subLast `T `true> t1 ->
     Typed ctx <`subLast `T `false> t2 ->
     Typed ctx <`subLast `T `cond> <`ifexpr `cond `t1 `t2>
-(*
 | ty_Empty : forall ctx, Typed ctx <`U> Empty
- *)
 | ty_Bool : forall ctx, Typed ctx <`U> Bool
 | ty_pi : forall ctx A B,
     Typed ctx <`U> A
-    -> Typed <`cons `ctx `A> <`U> B -> Typed ctx <`U> <`pi `A `B>
-.
+    -> Typed <`cons `ctx `A> <`U> B -> Typed ctx <`U> <`pi `A `B>.
 
 Ltac solve_no_unfold := repeat (lambda_solve ; repeat neutral_inj_case ;lambda_solve
                   ; repeat fast_neutral_unequal_case). 
@@ -74,445 +62,187 @@ Ltac solve_no_unfold := repeat (lambda_solve ; repeat neutral_inj_case ;lambda_s
 Ltac solve_all := repeat (unfold_all ; lambda_solve ; repeat neutral_inj_case ;lambda_solve
                   ; repeat fast_neutral_unequal_case). 
 
-
-(* The identity function is typed at U -> U*)
-Theorem test1 : Typed nil <`pi `Bool `Bool> <`lambda `zero>.
-(*Theorem test1 : Typed nil <`pi (fun env => asdf) (fun env => asdf)> <`lambda `zero>.*)
-Proof.
-  apply ty_lambda.
-  apply ty_pi.
-  apply ty_Bool.
-  apply ty_Bool.
-  apply ty_var.
-  Check ty_zero.
-  apply_cast ty_zero.
-  unfold_all.
-  lambda_solve.
-Qed.
-
 Inductive In': QTerm -> (QTerm -> Prop) -> Prop:=
-| in_Pi : forall (S : QTerm -> Prop) (F : forall a, (*S a ->*) QTerm -> Prop) A B,
+| in_Pi : forall (S : QTerm -> Prop) (F : QTerm -> (QTerm -> Prop)) A B,
     In' A S
-    -> (forall a (s : S a), In' <`B `a> (F a (*s*)))
-    -> In' <Pi `A `B> (fun f => forall a (s : S a), F a (*s*) <`f `a>)
+    -> (forall a, S a -> In' <`B `a> (F a))
+    -> In' <Pi `A `B> (fun f => forall a (s : S a), F a <`f `a>)
 | in_Bool :  In' <Bool> (fun b => b = <fun x => proj1 x> \/ b = <fun x => proj2 x>)
-| in_Empty : In' <Empty> (fun _ => False)
-.
+| in_Empty : In' <Empty> (fun _ => False).
 
 Inductive In : QTerm -> (QTerm -> Prop) -> Prop :=
 | in' : forall T S, In' T S -> In T S
-| in_type : In <U> (fun T => exists S, In' T S)
-.
-
-Require Import FunctionalExtensionality.
-Require Import Coq.Logic.PropExtensionality.
+| in_type : In <U> (fun T => exists S, In' T S).
 
 Theorem In_function : forall T S1 S2, In T S1 -> In T S2 -> S1 = S2.
-Proof.
+Proof with (try (intros; inversion H; inversion H0; solve_all; reflexivity; fail)).
   intros T S1 S2 in1.
-  generalize S2.
-  clear S2.
-  induction in1 as [T S in1 | typeCase].
-  induction in1 as [ S F A B In_A_S In_A_S_only In_Ba_Fa In_Ba_Fa_only | | ].
-  - intros S2 in2.
-    inversion in2 as [T S'' in2' | ].
-    inversion in2' as [S' F' A' B' In_A_S' In_Ba_F'a eq extra | | ].
-    + (* Pi Pi *)
-      solve_all.
-      clear extra.
-      clear in2.
-      (*clear S''.*)
-      specialize (In_A_S_only S' (in' _ _ In_A_S')).
-      subst S'.
-
-      assert (forall a, S a -> F a = F' a).
-      {
-        intros.
-        apply In_Ba_Fa_only.
-        apply H.
-        apply in'.
-        apply In_Ba_F'a.
-        apply H.
-      }
-      apply functional_extensionality.
-      intros f.
-      apply propositional_extensionality.
-      split.
-      * intros hyp a Sa.
-        rewrite <- H.
-        apply hyp.
-        apply Sa.
-        apply Sa.
-      * intros hyp a Sa.
-        rewrite H.
-        apply hyp.
-        apply Sa.
-        apply Sa.
-    + (* Pi Bool *) solve_all.
-    +  (* Pi EMpty *) solve_all.
-    + (* Pi Type *) solve_all.
-  - intros.
-    inversion H.
-    inversion H0.
-    * (* Bool Pi *) solve_all.
-    * (* Bool Bool *) solve_all.
-    * (* Bool Empty *) solve_all.
-    * (* Bool Type *) solve_all.
-  - intros.
-    inversion H.
-    inversion H0.
-    * (* Empty Pi *) solve_all.
-    * (* Empty Bool *) solve_all.
-    * (* Empty Empty *) solve_all.
-    * (* Empty Type *) solve_all.
+  generalize dependent S2.
+  destruct in1 as [T S in1 | typeCase].
+  - induction in1 as [ S F A B In_A_S In_A_S_only In_Ba_Fa In_Ba_Fa_only | | ]...
+    intros S2 in2.
+    inversion in2 as [T S'' in2' | ]; solve_all.
+    inversion in2' as [S' F' A' B' In_A_S' In_Ba_F'a eq extra | | ]; solve_all.
+    solve_all.
+    rewrite (In_A_S_only S' (in' _ _ In_A_S')) in *.
+    subst.
+    extensionality f.
+    extensionality a.
+    extensionality Sa.
+    rewrite (In_Ba_Fa_only a Sa (F' a) (in' _ _ (In_Ba_F'a a Sa))).
+    reflexivity.
   - intros.
     inversion H.
     inversion H0; solve_all. (* Type x anything cases*)
     reflexivity. (* Type Type case*)
 Qed.
 
-(* Will this work? In contrast to the logical relation itself, this is QTerm -> QTerm -> Prop
-instead of QTerm -> (QTerm -> Prop) -> Prop. This seems to correspond to Yiyun's paper. *)
-(* first arg env, second arg ctx. Idk why I did it like that, its opposite other conventions
-in this file. *)
 Inductive InCtx : QTerm -> QTerm -> Prop :=
 | in_nil : InCtx nil nil
 | in_cons : forall env ctx val T S,
     InCtx env ctx
     -> In <`T `env> S
     -> S val
-    -> InCtx <`env , `val> <`cons `ctx `T> 
-.
+    -> InCtx <`env , `val> <`cons `ctx `T>.
 
-Theorem fundamental_lemma_for_variables : forall ctx T t env,
-    VarTyped ctx T t -> InCtx env ctx -> exists S, In <`T `env> S /\ S <`t `env>.
-Proof.
-  intros.
-  generalize env, H0.
-  clear H0.
-  clear env.
-  induction H.
-  -
-    intros env inctx.
-    inversion inctx.
-    + solve_all.
-    +
-      solve_all.
-      exists S.
-      split.
-      assumption.
-      assumption.
-  - intros.
-    inversion H0.
-    + solve_all.
-    + solve_all.
-      apply IHVarTyped.
-      apply H2.
-Qed.
 
 Theorem fundamental_lemma : forall ctx T t env,
-    Typed ctx T t (*-> InCtx env ctx -> *)
+    Typed ctx T t
     -> InCtx env ctx
     -> exists S, In <`T `env> S
     /\ S <`t `env>.
 Proof.
   intros.
-  generalize H0.
-  generalize env.
-  clear H0.
-  clear env.
+  generalize dependent env.
   induction H.
   (* lambda *)
   - intros env inctx.
-    unfold pi.
-    normalize.
-    (* We need to show the "In (Pi ...) ..." from the goal by instantiating in_Pi.
-       but how can I get the In A _ argument needed? *)
-    Check in_Pi.
-    (* If I had that, could I do the rest?
-       In Yiyun's paper, he has that (Pi A B) is well typed in the lambda constructor.
-       For now, I will assume that as holes and see if the rest works. *)
-    specialize (IHTyped1 env inctx).
-    destruct IHTyped1 as [SU temp].
-    destruct temp as [InUPiAB SPiABPiAB].
-    inversion InUPiAB.
-    inversion H1; solve_all. (* can't be any of the non-U cases *)
-    rewrite <- H1 in SPiABPiAB.
-    destruct SPiABPiAB as [SPiAB In'PiAB].
-    inversion In'PiAB; try solve_all.
-    assert (In' <`A `env> S) as INA.
-    {
-      apply H4.
-    }
-    (*destruct H1 as [SA In_A_SA].*)
-    assert (forall a : QTerm, S a -> In' <`B (`env , `a)> (F a)) as In_Ba_Fa.
-    {
-      intros a sa.
-      specialize (H5 a sa).
-      normalize_in H5.
-      apply H5.
-    }
-    Check in_Pi.
-    Check (in_Pi S F <`A `env> <fun a => `B[a] (`env[a] , a)> H4).
-    (*assert (forall a, <(fun a => `B[a] (`env[a] , a)) `a> = <`B (`env , `a)>). { intros. lambda_solve.}*)
-    assert (forall a : QTerm, S a -> In' <(fun a => `B[a] (`env[a] , a)) `a> (F a)) as In_Ba_Fa_2.
-    {
-      intros.
-      lambda_solve.
-      apply In_Ba_Fa.
-      apply H2.
-    }
+    specialize (IHTyped1 env inctx) as [SU [InU piAB_in_SU]].
+    inversion InU; clear InU; subst; [inversion H1|]; solve_all.
+    destruct piAB_in_SU as [SPiAB In'PiAB].
+    inversion In'PiAB; clear In'PiAB; solve_all.
     exists (fun f : QTerm => forall a : QTerm, S a -> F a <`f `a>).
     split.
-    Check (in_Pi S F <`A `env> <fun a => `B[a] (`env[a] , a)> H4 In_Ba_Fa_2).
-    apply in'.
-    apply (in_Pi S F <`A `env> <fun a => `B[a] (`env[a] , a)> H4 In_Ba_Fa_2).
-    intros a SAa.
-    Check in_cons.
-    specialize (In_Ba_Fa a SAa).
-    (*Check (IHTyped2 <`env , `a> (in_cons _ _ _ _ S inctx (in' _ _ H4) SAa)).*)
-    Check in_cons.
-    specialize (IHTyped2 <`env , `a>).
-    assert (<cons `ctx `A> = <`cons `ctx `A>). unfold cons. normalize. reflexivity.
-    rewrite H2 in IHTyped2.
-    destruct (IHTyped2 (in_cons _ _ _ _ S inctx (in' _ _ INA) SAa)) as [Fa' temp].
-    destruct temp as [InBFa' Fa's].
-    unfold lambda.
-    normalize.
-    Check In_function.
-    rewrite (In_function _ _ _ (in' _ _ In_Ba_Fa) InBFa').
-    apply Fa's.
+    + repeat constructor; intros; eauto.
+    + intros a SAa.
+      specialize (H3 a SAa).
+      solve_all.
+      specialize (IHTyped2 <`env , `a>).
+      replace <cons `ctx `A> with <`cons `ctx `A> in IHTyped2 by (unfold cons; normalize; reflexivity).
+      destruct (IHTyped2 (in_cons _ _ _ _ S inctx (in' _ _ H2) SAa)) as [Fa' [InBFa' Fa's]].
+      rewrite (In_function _ _ _ (in' _ _ H3) InBFa').
+      apply Fa's.
   (* app *)
   - intros env inctx.
-    specialize (IHTyped1 env inctx).
-    specialize (IHTyped2 env inctx).
-    destruct IHTyped1 as [SPIAB temp].
-    destruct temp as [inPiAB s1Elem].
-    destruct IHTyped2 as [SA temp].
-    destruct temp as [inA s2Elem].
-    inversion inPiAB as [T S in'PiAB | TODOTODO ].
-    inversion in'PiAB as [ SA' F A' B' In_A'_SA' In_B'a_F'a eq | |].
-    (* The real case *)
-    +
-      unfold pi in eq.
-      solve_no_unfold.
-      assert (SA' = SA). {apply (In_function _ _ _ (in' _ _ In_A'_SA') inA).}
-      subst SA'.
-      exists (F <`s2 `env>).
-      specialize (In_B'a_F'a <`s2 `env> s2Elem).
-      normalize_in In_B'a_F'a.
-      split.
-      unfold subLast.
-      normalize.
-      apply in'.
+    specialize (IHTyped1 env inctx) as [SPIAB [inPiAB s1Elem]].
+    specialize (IHTyped2 env inctx) as [SA [inA s2Elem]].
+    inversion inPiAB as [T S in'PiAB |]; solve_all.
+    inversion in'PiAB as [ SA' F A' B' In_A'_SA' In_B'a_F'a eq | |]; solve_all; subst.
+    replace SA' with SA in * by (symmetry; apply (In_function _ _ _ (in' _ _ In_A'_SA') inA)).
+    exists (F <`s2 `env>).
+    specialize (In_B'a_F'a <`s2 `env> s2Elem).
+    specialize (s1Elem <`s2 `env> s2Elem).
+    normalize_in In_B'a_F'a.
+    split.
+    + apply in'.
       apply In_B'a_F'a.
-      rewrite <- H4 in s1Elem.
-      specialize (s1Elem <`s2 `env> s2Elem).
-      unfold app.
-      normalize.
-      apply s1Elem.
-    (* Its not Type *)
-    + solve_all.
-    (* Its not empty*)
-    + solve_all.
-    + solve_all.
+    + apply s1Elem.
   (* var *)
   - intros env inctx.
-    apply (fundamental_lemma_for_variables ctx T t env H inctx).
+    generalize dependent env.
+    induction H; intros x inctx; inversion inctx; solve_all; eauto.
   (* true *)
   - intros env inctx.
-    exists (fun b => b = <fun x => proj1 x> \/ b = <fun x => proj2 x>).
-    unfold Bool.
-    normalize.
-    split.
-    apply in'.
-    apply in_Bool.
-    apply or_introl.
+    eexists.
     solve_all.
+    split; repeat constructor; solve [solve_all].
   (* false *)
   - intros.
-    exists (fun b => b = <fun x => proj1 x> \/ b = <fun x => proj2 x>).
-    unfold Bool.
-    normalize.
-    split.
-    apply in'.
-    apply in_Bool.
-    apply or_intror.
+    eexists.
     solve_all.
+    split; repeat constructor; solve [solve_all].
   (* if *)
   - intros env inctx.
-    specialize (IHTyped1 env inctx).
-    destruct IHTyped1 as [S temp].
-    destruct temp as [In_Bool_S S_cond].
-    inversion In_Bool_S as [T0 S0' In_Bool_S' | TODOTODO ].
-    inversion In_Bool_S'.
-    (* Pi *)
-    + solve_all.
-    (* Bool *)
-    + rewrite <- H4 in S_cond.
-      destruct S_cond.
-      * (*true*)
-        specialize (IHTyped2 env inctx).
-        destruct IHTyped2 as [S0 temp].
-        destruct temp as [In_Ttrue_S0 S0_t1].
-        exists S0.
-        unfold subLast.
-        normalize.
-        unfold subLast, true in In_Ttrue_S0.
-        normalize_in In_Ttrue_S0.
-        rewrite H6.
-        split.
-        apply_cast In_Ttrue_S0.
-        solve_all.
-        (* TODO: make solve_all handle pairs! Then I can simplify this stuff. *)
-        assert (<fun p => proj1 p> = <fun x => proj1 x>). solve_all.
-        rewrite H2.
-        reflexivity.
-        unfold ifexpr.
-        normalize.
-        rewrite H6.
-        normalize.
+    specialize (IHTyped1 env inctx) as [S [In_Bool_S S_cond]].
+    inversion In_Bool_S as [T0 S0' In_Bool_S' | ]; solve_all.
+    inversion In_Bool_S'; solve_all.
+    subst.
+    destruct S_cond.
+    + (*true*)
+      specialize (IHTyped2 env inctx) as [S0 [In_Ttrue_S0 S0_t1]].
+      exists S0.
+      rewrite H2.
+      split.
+      * solve_all.
+        replace <fun p => proj1 p> with <fun x => proj1 x> in * by solve_all.
+        apply In_Ttrue_S0.
+      * normalize.
         apply S0_t1.
-      * (* false *)
-        specialize (IHTyped3 env inctx).
-        destruct IHTyped3 as [S0 temp].
-        destruct temp as [In_Ttrue_S0 S0_t1].
-        exists S0.
-        unfold subLast.
-        normalize.
-        unfold subLast, true in In_Ttrue_S0.
-        normalize_in In_Ttrue_S0.
-        rewrite H6.
-        split.
-        apply_cast In_Ttrue_S0.
-        solve_all.
-        (* TODO: make solve_all handle pairs! Then I can simplify this stuff. *)
-        assert (<fun p => proj2 p> = <fun x => proj2 x>). solve_all.
-        rewrite H2.
-        reflexivity.
-        unfold ifexpr.
-        normalize.
-        rewrite H6.
-        normalize.
+    + (* false *)
+      specialize (IHTyped3 env inctx) as [S0 [In_Tfalse_S0 S0_t1]].
+      exists S0.
+      rewrite H2.
+      split.
+      * solve_all.
+        replace <fun p => proj2 p> with <fun x => proj2 x> in * by solve_all.
+        apply In_Tfalse_S0.
+      * normalize.
         apply S0_t1.
-    (* Empty *)
-    + solve_all.
-    (* Type case *)
-    + solve_all.
-  (* Bool : Type *)
+  (* Empty *)
   - intros.
-    exists (fun T => exists S, In' T S).
-    unfold U. normalize.
-    Check in_type.
+    eexists.
+    solve_all.
     split.
-    apply in_type.
-    exists (fun b => b = <fun x => proj1 x> \/ b = <fun x => proj2 x>).
-    unfold Bool.
-    normalize.
-    apply in_Bool.
+    + apply in_type.
+    + eexists.
+      apply in_Empty.
+  (* Bool *)
+  - intros.
+    eexists.
+    solve_all.
+    split.
+    + apply in_type.
+    + eexists.
+      apply in_Bool.
   (* Pi : Type*)
   - intros env inctx.
-    Check in_Pi.
-    (*
-      To summarize, our induction hypotheses are that:
-      1) In any environment related to ctx, A has an interpreetation
-      2) In any environment related to (cons ctx A), B has an interpreetation
-      And we need to show that:
-         In an environment related to ctx, (Pi A B) has an interpretation.
-
-
-      I think that this should work, but we may need to modify in_Pi so that
-      instead of
-      F : QTerm -> QTerm -> Prop
-      we have
-      F : forall (a : QTerm), S a -> QTerm -> Prop.
-      I'm not sure yet if this is needed though.
-     *)
-    exists (fun T => exists S, In' T S).
-    unfold U. normalize.
-    split.
-    apply in_type.
-    specialize (IHTyped1 env inctx).
-    Check in_Pi.
-    destruct IHTyped1 as [SAU temp].
-    destruct temp as [InUSA SAA].
-    inversion InUSA.
-    inversion H1; solve_all.
-    rewrite <- H1 in SAA.
+    eexists.
+    unfold U.
+    normalize.
+    split; [apply in_type|].
+    specialize (IHTyped1 env inctx) as [SAU [InUSA SAA]].
+    inversion InUSA. {inversion H1; solve_all.}
+    subst.
     destruct SAA as [SA InASA].
-
-    pose (fun (a : QTerm) (sa : SA a) => IHTyped2 <`env, `a>
-                   (in_cons _ _ _ _ _ inctx (in' _ _ InASA) sa)) as thing.
-
-    Set Nested Proofs Allowed.
-    Lemma hasInterp : forall t env, (exists S, In <`U `env> S /\ S t) -> (exists S', In' t S').
-    Proof.
-      intros.
-      destruct H.
-      destruct H.
-      inversion H.
-      inversion H1; solve_all.
-      rewrite <- H1 in H0.
-      apply H0.
-    Defined.
-
-    pose (fun (a : QTerm) (sa : SA a) =>
-            hasInterp _ _ (IHTyped2 <`env, `a>
-                (in_cons _ _ _ _ _ inctx (in' _ _ InASA) sa))) as thing2.
-    
-    (*pose (fun (a : QTerm) (b : QTerm) => forall (sa : SA a),
-              match (thing2 a sa) with
-              | ex_intro _ SB _ => SB b
-              end) as F.*)
-    pose (fun (a b : QTerm) => exists SB, In' <`B (`env , `a)> SB /\ SB b) as F.
-    assert (forall a (s : SA a), In' <`B (`env ,`a)> (F a)).
-    {
-      intros a SAa.
-      destruct (thing2 a SAa) as [SB INBSB].
-      assert (F a = SB).
-      apply functional_extensionality.
-      intros b.
-      unfold F.
-      apply propositional_extensionality.
-      split.
-      intros.
-      destruct H3.
-      destruct H3.
-      rewrite <- (In_function _ _ _ (in' _ _ INBSB) (in' _ _ H3)) in H4.
-      assumption.
-      intros SBb.
-      exists SB.
-      split.
-      assumption.
-      assumption.
-      rewrite <- H3 in INBSB.
-      assumption.
-    }
-    assert (forall a : QTerm, SA a -> In' <(fun a => `B [a] (`env [a], a)) `a> (F a)).
-    {
-      intros a sa.
-      normalize.
-      apply H3.
-      apply sa.
-    }
-
-    Check in_cons.
-    Check (in_cons _ _ _ _ _ inctx (in' _ _ InASA)).
-    Check (in_Pi SA F <`A `env> <fun a => `B[a] (`env[a] , a)> InASA H4).
-    exists (fun f : QTerm => forall a : QTerm, SA a -> F a <`f `a>).
     unfold pi.
     normalize.
-    apply (in_Pi SA F <`A `env> <fun a => `B[a] (`env[a] , a)> InASA H4).
+    eexists.
+    pose (fun (a b : QTerm) => exists SB, In' <`B (`env , `a)> SB /\ SB b) as F.
+    apply in_Pi with (F := F); eauto.
+
+    intros.
+    specialize (IHTyped2 <`env, `a> (in_cons _ _ _ _ _ inctx (in' _ _ InASA) H1)) as [SU [InUS BinSU]].
+    solve_all.
+    rewrite <- (In_function _ _ _ InUSA InUS) in BinSU.
+    destruct BinSU as [SB In'BSB].
+
+    replace SB with ((fun _ => SB) a) in In'BSB by reflexivity.
+    replace (F a) with SB; auto.
+    unfold F.
+    extensionality b.
+    apply propositional_extensionality.
+    split; intros; eauto.
+    destruct H2.
+    destruct H2.
+    rewrite (In_function _ _ _ (in' _ _ In'BSB) (in' _ _ H2)).
+    auto.
 Qed.
      
-Theorem consistency : forall t,
-    Typed nil Empty t -> False.
+Theorem consistency : forall t, Typed nil Empty t -> False.
 Proof.
   intros.
-  pose (fundamental_lemma nil Empty t nil H in_nil) as x.
-  destruct x.
-  destruct H0.
-  inversion H0; inversion H2; solve_all.
-  rewrite <- H5 in H1.
-  assumption.
+  destruct (fundamental_lemma nil Empty t nil H in_nil) as [S [InEmptyS H1]].
+  inversion InEmptyS; inversion H0; solve_all.
+  subst.
+  auto.
 Qed.
